made progress in reasoning principles for convergence

theories/Dijkstra/IterRel.v
@@ -1,5 +1,8 @@
 From Coq Require Import Logic.Classical_Prop.
 From Paco Require Import paco.
+From Coq Require Import Init.Wf.
+From Coq Require Import Arith.Wf_nat.
+From Coq Require Import Program.Equality.
 Require Import Omega.
 Section IterRel.
 
@@ -77,6 +80,8 @@ Section IterRel.
     - auto using H1.
     - right. apply CIH. eapply H0; eauto.
   Qed.
+  (**)
+
 
   Lemma intro_wf : forall (P : A-> Prop) (m : A -> nat) (a : A),
       P a -> (forall a1 a2, P a1 -> r a1 a2 -> P a2 ) -> 
@@ -95,12 +100,97 @@ Section IterRel.
   
 End IterRel.
 
-Lemma no_inf_dec_seq_aux : forall  (r : nat -> nat -> Prop) (n n': nat),
-    n' <= n ->
-    (forall n1 n2, r n1 n2 -> n2 < n1) ->
-     wf_from nat r n -> wf_from nat r n'.
-  Proof.
-    intros. generalize dependent n'. 
-    induction H1 as [n Hn| n Hn].
-    - 
-        Abort.
+Definition rel_rev {A : Type} (r : A -> A -> Prop) : A -> A -> Prop := fun a0 a1 => r a1 a0.
+
+(*note that my notion of well_founded is sort of reverse of theres*)
+Lemma well_found_wf_from : forall (A : Type) (r : A -> A -> Prop), 
+    well_founded (rel_rev r) -> forall a, wf_from A r a.
+Proof.
+  intros A r Hwf a. unfold well_founded in Hwf.
+  unfold rel_rev in *. induction (Hwf a). apply step. intros.
+  apply H0 in H1. auto.
+Qed.
+
+(*Less than is well founded*)
+
+(*my well founded should be closed under subrelation*)
+
+Lemma wf_from_sub_rel : forall (A : Type) (r0 r1 : A -> A -> Prop) (a : A),
+    subrelation r0 r1 -> wf_from A r1 a -> wf_from A r0 a.
+Proof.
+  intros. induction H0.
+  - apply base. intros a' Hcontra. apply H in Hcontra. eapply H0; eauto.
+  - apply step. intros a' Hr0aa'. apply H in Hr0aa'. auto.
+Qed.
+
+Lemma wf_from_gt : forall (n : nat), wf_from nat (fun n0 n1 => n0 > n1) n.
+Proof.
+  intros.
+  enough (forall n', n' <= n -> wf_from nat (fun n0 n1 => n0 > n1) n' ); auto.
+  induction n; intros.
+  - assert (n' = 0); try omega. subst. apply base. intros. omega.
+  - apply step. intros n'' Hn''. assert (n'' <= n); try omega. auto.
+Qed.
+(*induct on f a*)
+Lemma no_inf_dec_seq_aux : forall  (r : nat -> nat -> Prop) (n: nat),
+    (forall n1 n2, r n1 n2 -> n1 > n2) ->
+     wf_from nat r n.
+Proof.
+  intros. eapply wf_from_sub_rel; try apply wf_from_gt. 
+  repeat intro. auto.
+Qed.
+
+(*Possibly uses some kind of transitivity in > that is missing in my more general proofs,
+  a more general proof would be nice but I think the nat*)
+Lemma wf_intro_gt : forall (A : Type) (r : A -> A -> Prop) (f : A -> nat) (P : A -> Prop) (a : A),
+    (forall a1 a2, P a1 -> r a1 a2 -> P a2) -> 
+    (forall a1 a2, P a1 -> r a1 a2 -> f a1 > f a2) -> 
+    P a -> wf_from A r a.
+Proof.
+  intros A r f inv a Hinv Hgt Ha. 
+  remember (f a) as n0. 
+  generalize dependent a. 
+  enough (forall a, f a <= n0 -> inv a -> wf_from A r a).
+  {
+    intros. apply H. omega. auto.
+  }
+  induction n0; intros.
+  - apply base. assert (f a = 0); try omega. 
+    intros a' Hcontra. 
+    specialize (Hgt a a' H0 Hcontra). omega. 
+  - apply step. intros a' Ha'. 
+    apply IHn0; eauto.
+    assert (f a > f a'); eauto. omega.
+Qed.
+
+
+(*
+Definition injective {A B: Type} (r : A -> B -> Prop) := forall a, exists b, r a b.
+
+Lemma wf_intro_r : forall (A B : Type) (ra : A -> A -> Prop) (rb : B -> B -> Prop)
+                   (rab : A -> B -> Prop) (a : A) (b : B), 
+    injective rab ->
+    (forall a1 a2 b1 b2, ra a1 a2 -> rab a1 b1 -> rab a2 b2 -> rb b1 b2) ->
+    rab a b ->
+    wf_from B rb b -> wf_from A ra a.
+Proof.
+  intros. rename H into Hinj. rename H0 into Hresp. rename H1 into Hab.  rename H2 into Hb.
+  induction Hb.
+  - apply base. intros a' Ha'. rename a0 into b. destruct  (Hinj a') as [b' Hb']. 
+    apply H with (a' := b'). eapply Hresp; eauto.
+  - rename a0 into b. eapply H0; eauto.
+Abort.
+    (*maybe if I had a more general notion of subrelation where r0 and r1 can be different types*)
+ (*problem seems to be more fundamental than I thought*)
+    (*ultimately this theorem is about injecting one type into another and inferring stuff from the image*)
+    (*mayb rab must be injective*)
+
+Lemma wf_intro_f : forall (A B : Type) (ra : A -> A -> Prop) (rb : B -> B -> Prop)
+                   (f : A -> B) (a : A), (forall a1 a2, ra a1 a2 -> rb (f a1) (f a2) ) ->
+                   wf_from B rb (f a) -> wf_from A ra a.
+Proof.
+  intros. dependent induction H0.
+  - apply base. intros a' Hcontra. apply H0 with (a' := f a'). auto.
+  -eapply H0; auto.
+ Abort.
+*)
